unified theory for all logical auxiliary material

thys/Native_Word/Uint_Common.thy
@@ -1,18 +1,33 @@
-(*  Title:      Word_Type_Copies.thy
+(*  Title:      Uint_Common.thy
+    Author:     Andreas Lochbihler, ETH Zurich
     Author:     Florian Haftmann, TU Muenchen
 *)
 
-chapter \<open>Systematic approach towards type copies of word type\<close>
+chapter \<open>Common logic auxiliary for all fixed-width word types\<close>
 
-theory Word_Type_Copies
+theory Uint_Common
   imports
     "HOL-Library.Word"
+    "Word_Lib.Signed_Division_Word"
     "Word_Lib.Most_significant_bit"
-    "Word_Lib.Least_significant_bit"
     "Word_Lib.Generic_set_bit"
     "Word_Lib.Bit_Comprehension"
-    "Code_Target_Word_Base"
 begin
+
+section \<open>Some abstract nonsense\<close>
+
+lemmas [transfer_rule] =
+  identity_quotient
+  fun_quotient
+  Quotient_integer[folded integer.pcr_cr_eq]
+
+lemma undefined_transfer:
+  assumes "Quotient R Abs Rep T"
+  shows "T (Rep undefined) undefined"
+using assms unfolding Quotient_alt_def by blast
+
+bundle undefined_transfer = undefined_transfer[transfer_rule]
+
 
 section \<open>Establishing type class instances for type copies of word type\<close>
 
@@ -423,5 +438,307 @@ lemma generic_set_bit_code [code]:
      size_eq_length size_integer_eq_length set_bit_beyond word_size)
 
 end
+
+subsection \<open>Division by signed division\<close>
+
+text \<open>Division on @{typ "'a word"} is unsigned, but Scala and OCaml only have signed division and modulus.\<close>
+
+context
+begin
+
+private lemma div_half_nat:
+  fixes m n :: nat
+  assumes "n \<noteq> 0"
+  shows "(m div n, m mod n) = (
+    let
+      q = 2 * (drop_bit 1 m div n);
+      r = m - q * n
+    in if n \<le> r then (q + 1, r - n) else (q, r))"
+proof -
+  let ?q = "2 * (drop_bit 1 m div n)"
+  have q: "?q = m div n - m div n mod 2"
+    by (simp add: modulo_nat_def drop_bit_Suc, simp flip: div_mult2_eq add: ac_simps)
+  let ?r = "m - ?q * n"
+  have r: "?r = m mod n + m div n mod 2 * n"
+    by (simp add: q algebra_simps modulo_nat_def drop_bit_Suc, simp flip: div_mult2_eq add: ac_simps)
+  show ?thesis
+  proof (cases "n \<le> m - ?q * n")
+    case True
+    with assms q have "m div n mod 2 \<noteq> 0"
+      unfolding r by simp (metis add.right_neutral mod_less_divisor mult_eq_0_iff not_less not_mod2_eq_Suc_0_eq_0)
+    hence "m div n = ?q + 1" unfolding q
+      by simp
+    moreover have "m mod n = ?r - n" using \<open>m div n = ?q + 1\<close>
+      by (simp add: modulo_nat_def)
+    ultimately show ?thesis
+      using True by (simp add: Let_def)
+  next
+    case False
+    hence "m div n mod 2 = 0"
+      unfolding r by (simp add: not_le) (metis Nat.add_0_right assms div_less div_mult_self2 mod_div_trivial mult.commute)
+    hence "m div n = ?q"
+      unfolding q by simp
+    moreover have "m mod n = ?r" using \<open>m div n = ?q\<close>
+      by (simp add: modulo_nat_def)
+    ultimately show ?thesis
+      using False by (simp add: Let_def)
+  qed
+qed
+
+private lemma div_half_word:
+  fixes x y :: "'a :: len word"
+  assumes "y \<noteq> 0"
+  shows "(x div y, x mod y) = (
+    let
+      q = push_bit 1 (drop_bit 1 x div y);
+      r = x - q * y
+    in if y \<le> r then (q + 1, r - y) else (q, r))"
+proof -
+  obtain n where n: "x = of_nat n" "n < 2 ^ LENGTH('a)"
+    by (rule that [of \<open>unat x\<close>]) simp_all
+  moreover obtain m where m: "y = of_nat m" "m < 2 ^ LENGTH('a)"
+    by (rule that [of \<open>unat y\<close>]) simp_all
+  ultimately have [simp]: \<open>unat (of_nat n :: 'a word) = n\<close> \<open>unat (of_nat m :: 'a word) = m\<close>
+    by (transfer, simp add: take_bit_of_nat take_bit_nat_eq_self_iff)+
+  let ?q = "push_bit 1 (drop_bit 1 x div y)"
+  let ?q' = "2 * (drop_bit 1 n div m)"
+  have "drop_bit 1 n div m < 2 ^ LENGTH('a)"
+    using n by (simp add: drop_bit_Suc) (meson div_le_dividend le_less_trans)
+  hence q: "?q = of_nat ?q'" using n m
+    by (auto simp add: drop_bit_eq_div word_arith_nat_div uno_simps take_bit_nat_eq_self unsigned_of_nat)
+  from assms have "m \<noteq> 0" using m by - (rule notI, simp)
+  from n have "?q' < 2 ^ LENGTH('a)"
+    by (simp add: drop_bit_Suc) (metis div_le_dividend le_less_trans less_mult_imp_div_less linorder_not_le mult.commute)
+  moreover
+  have "2 * (drop_bit 1 n div m) * m < 2 ^ LENGTH('a)"
+    using n by (simp add: drop_bit_Suc ac_simps flip: div_mult2_eq)
+      (metis le_less_trans mult.assoc times_div_less_eq_dividend)
+  moreover have "2 * (drop_bit 1 n div m) * m \<le> n"
+    by (simp add: drop_bit_Suc flip: div_mult2_eq ac_simps)
+  ultimately
+  have r: "x - ?q * y = of_nat (n - ?q' * m)"
+    and "y \<le> x - ?q * y \<Longrightarrow> of_nat (n - ?q' * m) - y = of_nat (n - ?q' * m - m)"
+    using n m unfolding q
+     apply simp_all
+    apply (cases \<open>LENGTH('a) \<ge> 2\<close>)
+     apply (simp_all add: word_le_nat_alt take_bit_nat_eq_self unat_sub_if' unat_word_ariths unsigned_of_nat)
+    done
+  then show ?thesis using n m div_half_nat [OF \<open>m \<noteq> 0\<close>, of n] unfolding q
+    by (simp add: word_le_nat_alt word_div_def word_mod_def Let_def take_bit_nat_eq_self unsigned_of_nat
+      flip: zdiv_int zmod_int
+      split del: if_split split: if_split_asm)
+qed
+
+
+text \<open>
+  This algorithm implements unsigned division in terms of signed division.
+  Taken from Hacker's Delight.
+\<close>
+
+lemma divmod_via_sdivmod:
+  fixes x y :: "'a :: len word"
+  assumes "y \<noteq> 0"
+  shows "(x div y, x mod y) = (
+    if push_bit (LENGTH('a) - 1) 1 \<le> y then
+      if x < y then (0, x) else (1, x - y)
+    else let
+      q = (push_bit 1 (drop_bit 1 x sdiv y));
+      r = x - q * y
+    in if y \<le> r then (q + 1, r - y) else (q, r))"
+proof (cases "push_bit (LENGTH('a) - 1) 1 \<le> y")
+  case True
+  note y = this
+  show ?thesis
+  proof (cases "x < y")
+    case True
+    with y show ?thesis
+      by (simp add: word_div_less mod_word_less)
+  next
+    case False
+    obtain n where n: "y = of_nat n" "n < 2 ^ LENGTH('a)"
+      by (rule that [of \<open>unat y\<close>]) simp_all
+    have "unat x < 2 ^ LENGTH('a)" by (rule unsigned_less)
+    also have "\<dots> = 2 * 2 ^ (LENGTH('a) - 1)"
+      by(metis Suc_pred len_gt_0 power_Suc One_nat_def)
+    also have "\<dots> \<le> 2 * n" using y n
+      by transfer (simp add: take_bit_eq_mod)
+    finally have div: "x div of_nat n = 1" using False n
+      by (simp add: take_bit_nat_eq_self unsigned_of_nat word_div_eq_1_iff)
+    moreover have "x mod y = x - x div y * y"
+      by (simp add: minus_div_mult_eq_mod)
+    with div n have "x mod y = x - y" by simp
+    ultimately show ?thesis using False y n by simp
+  qed
+next
+  case False
+  note y = this
+  obtain n where n: "x = of_nat n" "n < 2 ^ LENGTH('a)"
+    by (rule that [of \<open>unat x\<close>]) simp_all
+  hence "int n div 2 + 2 ^ (LENGTH('a) - Suc 0) < 2 ^ LENGTH('a)"
+    by (cases \<open>LENGTH('a)\<close>)
+      (auto dest: less_imp_of_nat_less [where ?'a = int])
+  with y n have "sint (drop_bit 1 x) = uint (drop_bit 1 x)"
+    by (cases \<open>LENGTH('a)\<close>)
+      (auto simp add: sint_uint drop_bit_eq_div take_bit_nat_eq_self uint_div_distrib
+        signed_take_bit_int_eq_self_iff unsigned_of_nat)
+  moreover have "uint y + 2 ^ (LENGTH('a) - Suc 0) < 2 ^ LENGTH('a)"
+    using y by (cases \<open>LENGTH('a)\<close>)
+      (simp_all add: not_le word_less_alt uint_power_lower)
+  then have "sint y = uint y"
+    apply (cases \<open>LENGTH('a)\<close>)
+     apply (auto simp add: sint_uint signed_take_bit_int_eq_self_iff)
+    using uint_ge_0 [of y]
+    by linarith 
+  ultimately show ?thesis using y
+    apply (subst div_half_word [OF assms])
+    apply (simp add: sdiv_word_def signed_divide_int_def flip: uint_div)
+    done
+qed
+
+end
+
+
+subsection \<open>Conversion from \<^typ>\<open>int\<close> to \<^typ>\<open>'a word\<close>\<close>
+
+lemma word_of_int_via_signed:
+  includes bit_operations_syntax
+  assumes shift_def: "shift = push_bit LENGTH('a) 1"
+  and overflow_def:"overflow = push_bit (LENGTH('a) - 1) 1"
+  shows
+  "(word_of_int i :: 'a :: len word) =
+   (let i' = i AND mask LENGTH('a)
+    in if bit i' (LENGTH('a) - 1) then
+         if i' - shift < - overflow \<or> overflow \<le> i' - shift then arbitrary1 i' else word_of_int (i' - shift)
+       else if i' < - overflow \<or> overflow \<le> i' then arbitrary2 i' else word_of_int i')"
+proof -
+  define i' where "i' = i AND mask LENGTH('a)"
+  have "shift = mask LENGTH('a) + 1" unfolding assms
+    by (simp add: mask_eq_exp_minus_1) 
+  hence "i' < shift"
+    by (simp add: i'_def)
+  show ?thesis
+  proof(cases "bit i' (LENGTH('a) - 1)")
+    case True
+    then have unf: "i' = overflow OR i'"
+      apply (simp add: assms i'_def flip: take_bit_eq_mask)
+      apply (rule bit_eqI)
+      apply (auto simp add: bit_take_bit_iff bit_or_iff bit_exp_iff)
+      done
+    have \<open>overflow \<le> overflow OR i'\<close>
+      by (simp add: i'_def or_greater_eq)
+    then have "overflow \<le> i'"
+      by (subst unf)
+    hence "i' - shift < - overflow \<longleftrightarrow> False" unfolding assms
+      by(cases "LENGTH('a)")(simp_all add: not_less)
+    moreover
+    have "overflow \<le> i' - shift \<longleftrightarrow> False" using \<open>i' < shift\<close> unfolding assms
+      by(cases "LENGTH('a)")(auto simp add: not_le elim: less_le_trans)
+    moreover
+    have "word_of_int (i' - shift) = (word_of_int i :: 'a word)" using \<open>i' < shift\<close>
+      by (simp add: i'_def shift_def word_of_int_eq_iff flip: take_bit_eq_mask)
+    ultimately show ?thesis using True by(simp add: Let_def i'_def)
+  next
+    case False
+    have "i' = i AND mask (LENGTH('a) - 1)"
+      apply (rule bit_eqI)
+      apply (use False in \<open>auto simp add: bit_simps assms i'_def\<close>)
+      apply (auto simp add: less_le)
+      done
+    also have "\<dots> \<le> Bit_Operations.mask (LENGTH('a) - 1)"
+      using AND_upper2 mask_nonnegative_int by blast
+    also have "\<dots> < overflow"
+      by (simp add: mask_int_def overflow_def)
+    also
+    have "- overflow \<le> 0" unfolding overflow_def by simp
+    have "0 \<le> i'" by (simp add: i'_def)
+    hence "- overflow \<le> i'" using \<open>- overflow \<le> 0\<close> by simp
+    moreover
+    have "word_of_int i' = (word_of_int i :: 'a word)"
+      by (simp add: i'_def of_int_and_eq of_int_mask_eq)
+    ultimately show ?thesis using False by(simp add: Let_def i'_def)
+  qed
+qed
+
+
+subsection \<open>Quickcheck conversion functions\<close>
+
+context
+  includes state_combinator_syntax
+begin
+
+definition qc_random_cnv ::
+  "(natural \<Rightarrow> 'a::term_of) \<Rightarrow> natural \<Rightarrow> Random.seed
+    \<Rightarrow> ('a \<times> (unit \<Rightarrow> Code_Evaluation.term)) \<times> Random.seed"
+  where "qc_random_cnv a_of_natural i = Random.range (i + 1) \<circ>\<rightarrow> (\<lambda>k. Pair (
+       let n = a_of_natural k
+       in (n, \<lambda>_. Code_Evaluation.term_of n)))"
+
+end
+
+definition qc_exhaustive_cnv :: "(natural \<Rightarrow> 'a) \<Rightarrow> ('a \<Rightarrow> (bool \<times> term list) option)
+  \<Rightarrow> natural \<Rightarrow> (bool \<times> term list) option"
+where
+  "qc_exhaustive_cnv a_of_natural f d =
+   Quickcheck_Exhaustive.exhaustive (%x. f (a_of_natural x)) d"
+
+definition qc_full_exhaustive_cnv ::
+  "(natural \<Rightarrow> ('a::term_of)) \<Rightarrow> ('a \<times> (unit \<Rightarrow> term) \<Rightarrow> (bool \<times> term list) option)
+  \<Rightarrow> natural \<Rightarrow> (bool \<times> term list) option"
+where
+  "qc_full_exhaustive_cnv a_of_natural f d = Quickcheck_Exhaustive.full_exhaustive
+  (%(x, xt). f (a_of_natural x, %_. Code_Evaluation.term_of (a_of_natural x))) d"
+
+declare [[quickcheck_narrowing_ghc_options = "-XTypeSynonymInstances"]]
+
+definition qc_narrowing_drawn_from :: "'a list \<Rightarrow> integer \<Rightarrow> _"
+where
+  "qc_narrowing_drawn_from xs =
+   foldr Quickcheck_Narrowing.sum (map Quickcheck_Narrowing.cons (butlast xs)) (Quickcheck_Narrowing.cons (last xs))"
+
+locale quickcheck_narrowing_samples =
+  fixes a_of_integer :: "integer \<Rightarrow> 'a \<times> 'a :: {partial_term_of, term_of}"
+  and zero :: "'a"
+  and tr :: "typerep"
+begin
+
+function narrowing_samples :: "integer \<Rightarrow> 'a list"
+where
+  "narrowing_samples i =
+   (if i > 0 then let (a, a') = a_of_integer i in narrowing_samples (i - 1) @ [a, a'] else [zero])"
+by pat_completeness auto
+termination including integer.lifting
+proof(relation "measure nat_of_integer")
+  fix i :: integer
+  assume "0 < i"
+  thus "(i - 1, i) \<in> measure nat_of_integer"
+    by simp(transfer, simp)
+qed simp
+
+definition partial_term_of_sample :: "integer \<Rightarrow> 'a"
+where
+  "partial_term_of_sample i =
+  (if i < 0 then undefined
+   else if i = 0 then zero
+   else if i mod 2 = 0 then snd (a_of_integer (i div 2))
+   else fst (a_of_integer (i div 2 + 1)))"
+
+lemma partial_term_of_code:
+  "partial_term_of (ty :: 'a itself) (Quickcheck_Narrowing.Narrowing_variable p t) \<equiv>
+    Code_Evaluation.Free (STR ''_'') tr"
+  "partial_term_of (ty :: 'a itself) (Quickcheck_Narrowing.Narrowing_constructor i []) \<equiv>
+   Code_Evaluation.term_of (partial_term_of_sample i)"
+by (rule partial_term_of_anything)+
+
+end
+
+lemmas [code] =
+  quickcheck_narrowing_samples.narrowing_samples.simps
+  quickcheck_narrowing_samples.partial_term_of_sample_def
+
+
+subsection \<open>Code generator setup\<close>
+
+code_identifier code_module Uint_Common \<rightharpoonup>
+  (SML) Word and (Haskell) Word and (OCaml) Word and (Scala) Word
 
 end
