thys/Native_Word/Uint64.thy
@@ -5,8 +5,9 @@
 chapter \<open>Unsigned words of 64 bits\<close>
 
 theory Uint64 imports
-  Word_Type_Copies
+  Uint_Common
   Code_Target_Word
+  Code_Int_Integer_Conversion
   Code_Target_Integer_Bit
 begin
 
